added parameter to Picinae_calling.v so that it could be integrated cleanly with Picinae_simplifier_exps.v, then did most of the integration

Picinae_calling.v
@@ -52,6 +52,7 @@ Open Scope N.
 
 Module Type PICINAE_TRACING_DEFS (IL: PICINAE_IL).
   Import IL.
+  Parameter abspar : Type.
   Parameter absenv : Type.
 
   Parameter absleb : absenv -> absenv -> bool.
@@ -60,13 +61,14 @@ Module Type PICINAE_TRACING_DEFS (IL: PICINAE_IL).
   Parameter absenv_bind : absenv -> var -> exp -> absenv.
   Parameter absenv_meet : absenv -> absenv -> absenv.
 
-  Parameter absenv_models : hdomain -> absenv -> store -> store -> Prop.
+  Parameter absenv_models :
+    hdomain -> abspar -> absenv -> store -> store -> Prop.
 
   Axiom absenv_bind_models :
-    forall h st ae st' exp val v,
-      absenv_models h ae st st' ->
+    forall h ap st ae st' exp val v,
+      absenv_models h ap ae st st' ->
       eval_exp h st' exp val ->
-      absenv_models h (absenv_bind ae v exp) st (st' [v := val]).
+      absenv_models h ap (absenv_bind ae v exp) st (st' [v := val]).
 
   Axiom absleb_absle : forall e1 e2, absleb e1 e2 = true <-> absle e1 e2.
   Axiom absle_trans : forall e1 e2 e3 (HE1 : absle e1 e2) (HE2 : absle e2 e3),
@@ -75,20 +77,22 @@ Module Type PICINAE_TRACING_DEFS (IL: PICINAE_IL).
   Axiom absle_meet_l : forall a1 a2, absle (absenv_meet a1 a2) a1.
   Axiom absle_meet_r : forall a1 a2, absle (absenv_meet a1 a2) a2.
   Axiom absle_models :
-    forall h st aenv1 aenv2 st',
+    forall h ap st aenv1 aenv2 st',
       absle aenv1 aenv2 ->
-      absenv_models h aenv2 st st' ->
-      absenv_models h aenv1 st st'.
+      absenv_models h ap aenv2 st st' ->
+      absenv_models h ap aenv1 st st'.
 End PICINAE_TRACING_DEFS.
 
 Module Type PICINAE_ABSEXP_ASSOC_DEFS (IL : PICINAE_IL).
   Import IL.
+  Parameter abspar : Type.
   Parameter absexp : Type.
 
   Parameter absexp_default : var -> absexp.
   Parameter absexp_meet : absexp -> absexp -> absexp.
   Parameter absexp_abstract : exp -> alist var absexp -> absexp.
-  Parameter absexp_models : hdomain -> store -> absexp -> value -> Prop.
+  Parameter absexp_models :
+    hdomain -> abspar -> store -> absexp -> value -> Prop.
 
   Parameter absexple : absexp -> absexp -> Prop.
   Parameter absexpleb : absexp -> absexp -> bool.
@@ -97,10 +101,10 @@ Module Type PICINAE_ABSEXP_ASSOC_DEFS (IL : PICINAE_IL).
     forall v a, absexp_abstract (Var v) a = assoc_def v a (absexp_default v).
 
   Axiom absexp_models_eval :
-    forall h st st' e val aenv,
-      (forall v, absexp_models h st (absexp_abstract (Var v) aenv) (st' v)) ->
+    forall h ap st st' e val aenv,
+      (forall v, absexp_models h ap st (absexp_abstract (Var v) aenv) (st' v)) ->
       eval_exp h st' e val ->
-      absexp_models h st (absexp_abstract e aenv) val.
+      absexp_models h ap st (absexp_abstract e aenv) val.
 
   Axiom absexpleb_absexple :
     forall e1 e2, absexpleb e1 e2 = true <-> absexple e1 e2.
@@ -113,21 +117,15 @@ Module Type PICINAE_ABSEXP_ASSOC_DEFS (IL : PICINAE_IL).
     forall a1 a2 al,
       absexple al a1 -> absexple al a2 -> absexple al (absexp_meet a1 a2).
   Axiom absexple_models :
-    forall h st e1 e2 v,
-      absexple e1 e2 -> absexp_models h st e2 v -> absexp_models h st e1 v.
-  Axiom absexple_abstract :
-    forall a1 a2 e,
-      (forall v,
-          absexple (absexp_abstract (Var v) a1)
-                   (absexp_abstract (Var v) a2)) ->
-      absexple (absexp_abstract e a1) (absexp_abstract e a2).
+    forall h ap st e1 e2 v,
+      absexple e1 e2 -> absexp_models h ap st e2 v -> absexp_models h ap st e1 v.
 End PICINAE_ABSEXP_ASSOC_DEFS.
 
 Module PICINAE_ABSEXP_ASSOC
        (IL : PICINAE_IL) (DEFS : PICINAE_ABSEXP_ASSOC_DEFS IL)
 <: PICINAE_TRACING_DEFS IL.
   Import IL.
-
+  Definition abspar := DEFS.abspar.
   Definition absexp := DEFS.absexp.
   Definition absenv := alist var absexp.
 
@@ -154,13 +152,13 @@ Module PICINAE_ABSEXP_ASSOC
   Definition absexp_abstract := DEFS.absexp_abstract.
   Definition absexp_models_eval := DEFS.absexp_models_eval.
 
-  Definition absenv_models h ae st st' :=
-    forall v, DEFS.absexp_models h st (alookup v ae) (st' v).
+  Definition absenv_models h ap ae st st' :=
+    forall v, DEFS.absexp_models h ap st (alookup v ae) (st' v).
 
-  Theorem absenv_bind_models h st ae st' exp val v
-          (HM : absenv_models h ae st st')
+  Theorem absenv_bind_models h ap st ae st' exp val v
+          (HM : absenv_models h ap ae st st')
           (HE : eval_exp h st' exp val) :
-    absenv_models h (absenv_bind ae v exp) st (st' [v := val]).
+    absenv_models h ap (absenv_bind ae v exp) st (st' [v := val]).
   Proof.
     intro v'.
     unfold absenv_bind,alookup.
@@ -212,10 +210,10 @@ Module PICINAE_ABSEXP_ASSOC
     apply DEFS.absexple_refl.
   Qed.
 
-  Theorem absle_models h st a1 a2 st'
+  Theorem absle_models h ap st a1 a2 st'
           (HL : absle a1 a2)
-          (HM : absenv_models h a2 st st') :
-    absenv_models h a1 st st'.
+          (HM : absenv_models h ap a2 st st') :
+    absenv_models h ap a1 st st'.
   Proof.
     intro v.
     specialize (HM v).
@@ -334,6 +332,7 @@ Next Obligation. Proof. decide equality. apply iseq. Defined.
 
 Module PICINAE_ABSEXP_OPTEXPEQ (IL : PICINAE_IL) <: PICINAE_ABSEXP_ASSOC_DEFS IL.
   Import IL.
+  Definition abspar := unit.
   Definition absexp := option exp.
   Definition absexp_default v := Some (Var v).
 
@@ -444,7 +443,7 @@ Module PICINAE_ABSEXP_OPTEXPEQ (IL : PICINAE_IL) <: PICINAE_ABSEXP_ASSOC_DEFS IL
       → eval_exp_na s e2 (VaN n2 w2)
       → eval_exp_na s (Concat e1 e2) (VaN (N.lor (N.shiftl n1 w2) n2) (w1 + w2)).
 
-  Definition absexp_models (h : hdomain) s oe val :=
+  Definition absexp_models (h : hdomain) (ap : unit) s oe val :=
     match oe with
     | Some e => eval_exp_na s e val
     | None => True
@@ -474,10 +473,10 @@ Module PICINAE_ABSEXP_OPTEXPEQ (IL : PICINAE_IL) <: PICINAE_ABSEXP_ASSOC_DEFS IL
     induction HE; econstructor; eassumption.
   Qed.
 
-  Theorem absexp_models_eval h s s' e val a
-          (HM : forall v, absexp_models h s (absexp_abstract (Var v) a) (s' v))
+  Theorem absexp_models_eval h ap s s' e val a
+          (HM : forall v, absexp_models h ap s (absexp_abstract (Var v) a) (s' v))
           (HE : eval_exp h s' e val) :
-    absexp_models h s (absexp_abstract e a) val.
+    absexp_models h ap s (absexp_abstract e a) val.
   Proof.
     unfold absexp_models.
     revert s a HM.
@@ -510,15 +509,16 @@ Module PICINAE_ABSEXP_OPTEXPEQ (IL : PICINAE_IL) <: PICINAE_ABSEXP_ASSOC_DEFS IL
     all: econstructor; eassumption.
   Qed.
 
-  Theorem absexp_nil_models h st v :
-      absexp_models h st (absexp_abstract (Var v) nil) (st v).
+  Theorem absexp_nil_models h ap st v :
+      absexp_models h ap st (absexp_abstract (Var v) nil) (st v).
   Proof.
     constructor.
   Qed.
 
-  Theorem absexp_bind_models h st v e1 e2 val a
-      (HM : absexp_models h st (absexp_abstract (Let v e1 e2) a) val) :
+  Theorem absexp_bind_models h ap st v e1 e2 val a
+      (HM : absexp_models h ap st (absexp_abstract (Let v e1 e2) a) val) :
     absexp_models h
+                  ap
                   st
                   (absexp_abstract e2 (assoc_cons v (absexp_abstract e1 a) a))
                   val.
@@ -569,41 +569,11 @@ Module PICINAE_ABSEXP_OPTEXPEQ (IL : PICINAE_IL) <: PICINAE_ABSEXP_ASSOC_DEFS IL
     destruct iseq; tauto.
   Qed.
 
-  Theorem absexple_models h st e1 e2 v
-          (HL : absexple e1 e2) (HE : absexp_models h st e2 v) :
-    absexp_models h st e1 v.
+  Theorem absexple_models h ap st e1 e2 v
+          (HL : absexple e1 e2) (HE : absexp_models h ap st e2 v) :
+    absexp_models h ap st e1 v.
   Proof.
     destruct e1,e2; simpl in *; subst; tauto.
-  Qed.
-
-  Theorem absexple_abstract a1 a2 e
-          (HA : forall v, absexple (assoc_def v a1 (absexp_default v))
-                                   (assoc_def v a2 (absexp_default v))) :
-    absexple (absexp_abstract e a1) (absexp_abstract e a2).
-  Proof.
-    unfold absexple.
-    revert a1 a2 HA.
-    induction e; simpl; intros a1 a2 HA.
-    {
-      apply HA.
-    }
-    7: {
-      apply IHe2.
-      intro v'.
-      unfold absexple,assoc_def.
-      repeat rewrite assoc_cons_lookup.
-      simpl.
-      destruct iseq; subst; [apply IHe1,HA|apply HA].
-    }
-    all: try tauto.
-    all:
-      repeat match goal with
-               [ H :
-                 forall _ _, _ -> match absexp_abstract ?e _ with _ => _ end |- _ ] =>
-                 specialize (H _ _ HA);
-                 destruct (absexp_abstract e a1),(absexp_abstract e a2);
-                 subst; try tauto
-             end; try tauto.
   Qed.
 End PICINAE_ABSEXP_OPTEXPEQ.
 
@@ -667,12 +637,8 @@ Module PICINAE_CALLING (IL: PICINAE_IL) (DEFS : PICINAE_TRACING_DEFS IL).
     | _ => skip
     end.
 
-  (* Definition absenv_models h d st st' := *)
-  (*   forall e val (HM : eval_exp h st' e val), *)
-  (*     absexp_models h st (absexp_abstract e d) val. *)
-
-  Definition trace_state_models_exit h '(ax,d) st st' x :=
-    absenv_models h d st st' /\
+  Definition trace_state_models_exit h ap '(ax,d) st st' x :=
+    absenv_models h ap d st st' /\
       match ax,x with
       | AEExn n,Raise n'
       | AELoc n,Exit n' => n = n'
@@ -680,81 +646,53 @@ Module PICINAE_CALLING (IL: PICINAE_IL) (DEFS : PICINAE_TRACING_DEFS IL).
       | _,_ => False
       end.
 
-  Definition trace_state_models_oexit h P ts st st' ox :=
+  Definition trace_state_models_oexit h ap P ts st st' ox :=
     match ox with
-    | Some x => trace_state_models_exit h ts st st' x
+    | Some x => trace_state_models_exit h ap ts st st' x
     | None => P ts
     end.
 
-  Definition trace_states_model h tsl st st' x :=
-    Exists (fun ts => trace_state_models_exit h ts st st' x) tsl.
+  Definition trace_states_model h ap tsl st st' x :=
+    Exists (fun ts => trace_state_models_exit h ap ts st st' x) tsl.
 
-  Definition trace_states_modelo h P tsl st st' ox :=
-    Exists (fun ts => trace_state_models_oexit h P ts st st' ox) tsl.
+  Definition trace_states_modelo h ap P tsl st st' ox :=
+    Exists (fun ts => trace_state_models_oexit h ap P ts st st' ox) tsl.
 
-  Definition info_models_loc h info n st st' :=
+  Definition info_models_loc h ap info n st st' :=
     match treeN_lookup info n with
-    | Some d => absenv_models h d st st'
+    | Some d => absenv_models h ap d st st'
     | None => False
     end.
 
-  Definition info_models_exit h info st st' x :=
+  Definition info_models_exit h ap info st st' x :=
     match x with
     | Raise _ => False
-    | Exit n => info_models_loc h info n st st'
+    | Exit n => info_models_loc h ap info n st st'
     end.
 
   Definition exec_inter_prog h p a st time1 st' a' time2 st'' x :=
     exec_prog h p a st time1 st' (Exit a') /\
       exec_prog h p a' st' time2 st'' x.
 
-  Definition trace_result_models_exit h '(info,tsl) st st' x :=
-    info_models_exit h info st st' x \/ trace_states_model h tsl st st' x.
+  Definition trace_result_models_exit h ap '(info,tsl) st st' x :=
+    info_models_exit h ap info st st' x \/ trace_states_model h ap tsl st st' x.
 
-  Definition trace_result_consistent h '(info,tsl) p st :=
+  Definition trace_result_consistent h ap '(info,tsl) p st :=
     forall st' a st'' x sz q
-           (HInfo : info_models_loc h info a st st')
+           (HInfo : info_models_loc h ap info a st st')
            (HE : exec_stmt h st' q st'' x)
            (HP : p st' a = Some (sz,q)),
-      trace_result_models_exit h (info,tsl) st st'' (exitof (a+sz) x).
+      trace_result_models_exit h ap (info,tsl) st st'' (exitof (a+sz) x).
 
-  Definition trace_inter_consistent h '((info,tsl1),tsl2) p st :=
-    trace_result_consistent h (info,tsl1 ++ tsl2) p st.
+  Definition trace_inter_consistent h ap '((info,tsl1),tsl2) p st :=
+    trace_result_consistent h ap (info,tsl1 ++ tsl2) p st.
 
-  (* Theorem absenv_models_match h d st st' : *)
-  (*   absenv_models h d st st' <-> *)
-  (*     forall v, *)
-  (*       match d[[v]] with *)
-  (*       | Some ev => eval_exp h st ev (st' v) *)
-  (*       | None => True *)
-  (*       end. *)
-  (* Proof. *)
-  (*   unfold absenv_models. *)
-  (*   split; intro HM; intro v; specialize (HM v). *)
-  (*   { *)
-  (*     destruct (d [[v]]); [|tauto]. *)
-  (*     apply HM,eq_refl. *)
-  (*   } *)
-  (*   { *)
-  (*     intros. *)
-  (*     rewrite HX in HM. *)
-  (*     assumption. *)
-  (*   } *)
-  (* Qed. *)
-
-  (* Theorem absenv_models_le h d1 d2 st st' *)
-  (*         (HL : absle d1 d2) (HM : absenv_models h st d2 st') : *)
-  (*   absenv_models h st d1 st'. *)
-  (* Proof. *)
-  (*   eapply absle_models; eassumption. *)
-  (* Qed. *)
-
-  Theorem trace_stmt_result' h P st st' st'' d q next ox
-          (HD : absenv_models h d st st')
+  Theorem trace_stmt_result' h ap P st st' st'' d q next ox
+          (HD : absenv_models h ap d st st')
           (HE : exec_stmt h st' q st'' ox)
           (HN : match ox with
                 | None =>
-                    forall d' (HND : absenv_models h d' st st''),
+                    forall d' (HND : absenv_models h ap d' st st''),
                       match next d' with
                       | Some tsl' => Exists P tsl'
                       | None => True
@@ -762,7 +700,7 @@ Module PICINAE_CALLING (IL: PICINAE_IL) (DEFS : PICINAE_TRACING_DEFS IL).
                 | Some x => True
                 end) :
     match trace_stmt q next d with
-    | Some tsl => trace_states_modelo h P tsl st st'' ox
+    | Some tsl => trace_states_modelo h ap P tsl st st'' ox
     | None => True
     end.
   Proof.
@@ -807,15 +745,15 @@ Module PICINAE_CALLING (IL: PICINAE_IL) (DEFS : PICINAE_TRACING_DEFS IL).
     }
   Qed.
 
-  Theorem trace_stmt_result h st st' st'' d q n ox tsl
-          (HD : absenv_models h d st st')
+  Theorem trace_stmt_result h ap st st' st'' d q n ox tsl
+          (HD : absenv_models h ap d st st')
           (HE : exec_stmt h st' q st'' ox)
           (HTS: trace_stmt q (trace_exit_res n) d = Some tsl) :
-    trace_states_model h tsl st st'' (exitof n ox).
+    trace_states_model h ap tsl st st'' (exitof n ox).
   Proof.
-    pose (P := fun ts => trace_state_models_exit h ts st st'' (Exit n)).
+    pose (P := fun ts => trace_state_models_exit h ap ts st st'' (Exit n)).
     assert
-      (HX := trace_stmt_result' h P st st' st'' d q (trace_exit_res n) ox).
+      (HX := trace_stmt_result' h ap P st st' st'' d q (trace_exit_res n) ox).
     rewrite HTS in HX.
     specialize (HX HD HE).
     destruct ox; apply HX; [tauto|].
@@ -827,16 +765,16 @@ Module PICINAE_CALLING (IL: PICINAE_IL) (DEFS : PICINAE_TRACING_DEFS IL).
     tauto.
   Qed.
 
-  Theorem trace_result_consistent_exec h info tsl p a st st' time st'' x
-          (HC : trace_result_consistent h (info,tsl) p st)
-          (HInfo : info_models_loc h info a st st')
+  Theorem trace_result_consistent_exec h ap info tsl p a st st' time st'' x
+          (HC : trace_result_consistent h ap (info,tsl) p st)
+          (HInfo : info_models_loc h ap info a st st')
           (HE : exec_prog h p a st' time st'' x) :
-    trace_result_models_exit h (info,tsl) st st'' x \/
+    trace_result_models_exit h ap (info,tsl) st st'' x \/
       exists time1 time2 st'x a',
         time = (time1 + time2)%nat /\
           exec_prog h p a st' time1 st'x (Exit a') /\
           exec_prog h p a' st'x time2 st'' x /\
-          trace_states_model h tsl st st'x (Exit a').
+          trace_states_model h ap tsl st st'x (Exit a').
   Proof.
     revert HInfo.
     induction HE; simpl; [tauto| |]; intro.
@@ -875,19 +813,19 @@ Module PICINAE_CALLING (IL: PICINAE_IL) (DEFS : PICINAE_TRACING_DEFS IL).
     }
   Qed.
 
-  Theorem trace_result_consistent_init h tsl p st :
-    trace_result_consistent h (treeN_nil,tsl) p st.
+  Theorem trace_result_consistent_init h ap tsl p st :
+    trace_result_consistent h ap (treeN_nil,tsl) p st.
   Proof.
     simpl.
     intros.
     destruct a; compute in HInfo; tauto.
   Qed.
 
-  Theorem trace_step_modelled h p st tn tsl tnd d n
+  Theorem trace_step_modelled h ap p st tn tsl tnd d n
           (HTN : treeN_lookup tn n = Some tnd)
           (HLE : absle tnd d)
-          (HPrev : trace_result_consistent h (tn,(AELoc n,d)::tsl) p st) :
-    trace_result_consistent h (tn,tsl) p st.
+          (HPrev : trace_result_consistent h ap (tn,(AELoc n,d)::tsl) p st) :
+    trace_result_consistent h ap (tn,tsl) p st.
   Proof.
     unfold trace_result_consistent in *.
     intros.
@@ -905,38 +843,38 @@ Module PICINAE_CALLING (IL: PICINAE_IL) (DEFS : PICINAE_TRACING_DEFS IL).
     eapply absle_models; eassumption.
   Qed.
 
-  (* Theorem trace_state_models_exit_promote_word h d n w st st' x *)
-  (*         (HM : trace_state_models_exit h (AEExp (Word n w)) st st' x) : *)
-  (*   trace_state_models_exit h (d, AELoc n) st st' x. *)
-  (* Proof. *)
-  (*   simpl in *. *)
-  (*   destruct HM as [? HM]. *)
-  (*   split; [assumption|]. *)
-  (*   destruct x; [|tauto]. *)
-  (*   symmetry. *)
-  (*   destruct HM as [? HM]. *)
-  (*   inversion HM; subst. *)
-  (*   reflexivity. *)
-  (* Qed. *)
+  Theorem trace_state_models_exit_promote_word h ap d n w st st' x
+    (HM : trace_state_models_exit h ap (AEExp (Word n w), d) st st' x) :
+    trace_state_models_exit h ap (AELoc n, d) st st' x.
+  Proof.
+    simpl in *.
+    destruct HM as [? HM].
+    split; [assumption|].
+    destruct x; [|tauto].
+    symmetry.
+    destruct HM as [? HM].
+    inversion HM; subst.
+    reflexivity.
+  Qed.
 
-  (* Theorem trace_step_promote_word h p st tn tsl d n w *)
-  (*         (HPrev : trace_result_consistent h (tn,(AEExp (Word n w),d)::tsl) p st) : *)
-  (*   trace_result_consistent h (tn,(d,AELoc n)::tsl) p st. *)
-  (* Proof. *)
-  (*   unfold trace_result_consistent in *. *)
-  (*   unfold trace_result_models_exit in *. *)
-  (*   intros. *)
-  (*   specialize (HPrev st' a st'' x sz q HInfo HE HP). *)
-  (*   unfold trace_states_model in *. *)
-  (*   rewrite Exists_cons in *. *)
-  (*   destruct HPrev as [?|[HPrev|?] ]; [tauto| |tauto]. *)
-  (*   right. *)
-  (*   left. *)
-  (*   eapply trace_state_models_exit_promote_word. *)
-  (*   eassumption. *)
-  (* Qed. *)
+  Theorem trace_step_promote_word h ap p st tn tsl d n w
+    (HPrev : trace_result_consistent h ap (tn,(AEExp (Word n w),d)::tsl) p st) :
+    trace_result_consistent h ap (tn,(AELoc n,d)::tsl) p st.
+  Proof.
+    unfold trace_result_consistent in *.
+    unfold trace_result_models_exit in *.
+    intros.
+    specialize (HPrev st' a st'' x sz q HInfo HE HP).
+    unfold trace_states_model in *.
+    rewrite Exists_cons in *.
+    destruct HPrev as [?|[HPrev|?] ]; [tauto| |tauto].
+    right.
+    left.
+    eapply trace_state_models_exit_promote_word.
+    eassumption.
+  Qed.
 
-  Theorem trace_step_stmt_consistent h p st tn d tsl tsl' n sz q
+  Theorem trace_step_stmt_consistent h ap p st tn d tsl tsl' n sz q
           (dm := match treeN_lookup tn n with
                  | None => d
                  | Some d' => absenv_meet d d'
@@ -944,8 +882,8 @@ Module PICINAE_CALLING (IL: PICINAE_IL) (DEFS : PICINAE_TRACING_DEFS IL).
           (HP : forall st' n, p st' n = p st n)
           (HTX : p st n = Some (sz,q))
           (HT : trace_stmt q (trace_exit_res (n + sz)) dm = Some tsl')
-          (HPrev : trace_result_consistent h (tn,(AELoc n,d)::tsl) p st) :
-    trace_inter_consistent h ((treeN_update tn n (Some dm),tsl),tsl') p st.
+          (HPrev : trace_result_consistent h ap (tn,(AELoc n,d)::tsl) p st) :
+    trace_inter_consistent h ap ((treeN_update tn n (Some dm),tsl),tsl') p st.
   Proof.
     unfold dm in *.
     clear dm.
@@ -999,12 +937,12 @@ Module PICINAE_CALLING (IL: PICINAE_IL) (DEFS : PICINAE_TRACING_DEFS IL).
     }
   Qed.
 
-  Theorem trace_step_models_consistent h p st tn tsl ts
+  Theorem trace_step_models_consistent h ap p st tn tsl ts
           (HP : forall st' n, p st' n = p st n)
-          (HPrev : trace_result_consistent h (tn,ts::tsl) p st) :
-    trace_inter_consistent h (step_trace (p st) (tn,tsl) ts) p st.
+          (HPrev : trace_result_consistent h ap (tn,ts::tsl) p st) :
+    trace_inter_consistent h ap (step_trace (p st) (tn,tsl) ts) p st.
   Proof.
-    assert (HSkip : trace_inter_consistent h ((tn,ts::tsl),nil) p st)
+    assert (HSkip : trace_inter_consistent h ap ((tn,ts::tsl),nil) p st)
       by (simpl; rewrite app_nil_r; assumption).
     simpl.
     destruct ts as [ae d].
